%!TeX root=../solnQCQI.tex

\chapter{Entropy and information}
\Textbf{11.1}
Fair coin:

\begin{align}
    H({1/2, 1/2}) = \left( - \frac{1}{2} \log \frac{1}{2} \right) \times 2 = 1
\end{align}


Fair die:
\begin{align}
    H(p) = \left( - \frac{1}{6} \log \frac{1}{6} \right) \times 6 = \log 6.
\end{align}


The entropy decreases if the coin or die is unfair.



\Textbf{11.2}

From assumption $I(pq) = I(p) + I(q)$.

\begin{align}
    \frac{\partial I(pq)}{\partial p} &= \frac{\partial I(p)}{\partial p} + 0 = \frac{\partial I(p)}{\partial p}\\
    \frac{\partial I(pq)}{\partial q} &= 0 + \frac{\partial I(q)}{\partial q} = \frac{\partial I(q)}{\partial q}
\end{align}


\begin{align}
    \frac{\partial I(pq)}{\partial p}
        &=  \frac{\partial I(pq)}{\partial (pq)} \frac{\partial (pq)}{\partial p}
        = q \frac{\partial I(pq)}{\partial(pq)}
    \Rightarrow \frac{\partial I(pq)}{\partial(pq)} = \frac{1}{q} \frac{\partial I(p)}{\partial p}\\
%
    \frac{\partial I(pq)}{\partial q}
        &=  \frac{\partial I(pq)}{\partial (pq)} \frac{\partial (pq)}{\partial q}
        = p \frac{\partial I(pq)}{\partial(pq)}
    \Rightarrow \frac{\partial I(pq)}{\partial(pq)} = \frac{1}{p} \frac{\partial I(q)}{\partial q}
\end{align}

Thus
\begin{align}
    \frac{1}{q} \frac{\partial I(p)}{\partial p} &= \frac{1}{p} \frac{\partial I(q)}{\partial q}\\
    \therefore~ p \frac{d I(p)}{d p} &= q \frac{d I(q)}{d q} ~~~\text{ for all } p,q \in [0,1].\\
\end{align}

Then $p (d I(p) / d p)$ is constant.

If $p (d I(p) / d p) = k$, $k \in \mathds{R}$.
Then $I(p) = k \ln p = k' \log p$ where $k' = k / \log e$.



\Textbf{11.3}
$H_{\text{bin}}(p) = - p\log p - (1-p) \log (1-p)$.

\begin{align}
    \frac{d H_{\text{bin}}(p)}{d p}
        &= \frac{1}{\ln 2} \left( - \log p - 1 + \log (1-p) + 1 \right)\\
        &= \frac{1}{\ln 2} \ln \frac{1-p}{p} = 0\\
    \Rightarrow \frac{1-p}{p} = 1\\
    \Rightarrow p = 1/2.
\end{align}


\Textbf{11.4}
\Textbf{11.5}

\begin{align}
    H\left( p(x,y) || p(x)p(y) \right)
        &= \sum_{x,y} p(x,y) \log \frac{p(x) p(y)}{p(x,y)}\\
        &= - H(p(x,y)) - \sum_{x,y} p(x,y) \log \left[ p(x)p(y) \right]\\
        &= - H(p(x,y)) - \sum_{x,y} p(x,y) \left[ \log p(x) + \log p(y) \right]\\
        &= - H(p(x,y)) - \sum_{x,y} p(x,y) \log p(x) - \sum_{x,y} p(x,y) \log p(y)\\
        &= - H(p(x,y)) - \sum_{x} p(x) \log p(x) - \sum_{y} p(y) \log p(y)\\
        &= - H(p(x,y)) + H(p(x)) + H(p(y))\\
        &= - H(X,Y) + H(X) + H(Y).
\end{align}

From the non-negativity of the relative entropy,
\begin{align}
    H(X) +  H(Y) - H(X,Y) \geq 0\\
    \therefore H(X) + H(Y) \geq H(X,Y).
\end{align}



\Textbf{11.6}
\begin{align}
    H(Y) + H (X, Y, Z) - H(X, Y) - H(Y, Z)  
        &= \sum_{x,y,z} p(x,y,z) \log \left( p(x,y)p(y,z)/p(y)p(x,y,z) \right) \\
        &\geq \frac{1}{\ln{2}} \sum_{x,y,z} p(x,y,z) \left[1-p(x,y)p(y,z)/p(y)p(x,y,z) \right] \\
        = \frac{1-1}{\ln{2}}
        = 0
\end{align}
The equality occurs if and only if $p(x,y)p(y,z)/p(y)p(x,y,z)=1$, which means a Markov chain condition of $Z \rightarrow Y \rightarrow X$; $p(x|y)=p(x|y,z)$ 
\Textbf{11.7}
\Textbf{11.8}
\Textbf{11.9}
\Textbf{11.10}
\Textbf{11.11}
\Textbf{11.12}
\Textbf{11.13}
\Textbf{11.14}
\Textbf{11.15}
\Textbf{11.16}
\Textbf{11.17}
\Textbf{11.18}
\Textbf{11.19}
\Textbf{11.20}
\Textbf{11.21}
\Textbf{11.22}
\Textbf{11.23}
\Textbf{11.24}
\Textbf{11.25}
\Textbf{11.26}

\Textbf{Problem 11.1}
\Textbf{Problem 11.2}
\Textbf{Problem 11.3}
\Textbf{Problem 11.4}
\Textbf{Problem 11.5}
